BoogieLang/Semantics.thy
@@ -16,7 +16,15 @@ lemma lit_val_elim:
  "\<lbrakk> \<And>b. v = LitV (LBool b) \<Longrightarrow> P; \<And>i. v = LitV (LInt i) \<Longrightarrow> P; \<And> a. v = AbsV a \<Longrightarrow> P \<rbrakk> \<Longrightarrow> P"
   by (metis lit.exhaust val.exhaust)
 
-type_synonym 'a nstate = "vname \<rightharpoonup> 'a val"
+type_synonym 'a named_state = "vname \<rightharpoonup> 'a val"
+
+record 'a active_nstate = 
+  old_global_state :: "'a named_state"
+  global_state :: "'a named_state" 
+  local_state :: "'a named_state"
+  binder_state :: "nat \<rightharpoonup> 'a val"
+
+type_synonym 'a nstate = "'a active_nstate"
 
 datatype 'a state = Normal "'a nstate" | Failure | Magic
 
@@ -28,7 +36,28 @@ type_synonym 'a fun_interp = "fname \<rightharpoonup> (ty list \<Rightarrow> 'a 
 
 (* type declarations *)
 type_synonym 'a fun_context = "fdecls \<times> 'a fun_interp"
-type_synonym var_context = vdecls
+
+(* (global variable declarations, local variable declarations) *)
+type_synonym var_context = "vdecls \<times> vdecls"
+
+fun lookup_var_ty :: "var_context \<Rightarrow> vname \<Rightarrow> ty option"
+  where 
+    "lookup_var_ty (Locals, Globals) x = 
+      (case (map_of Locals x) of Some res \<Rightarrow> Some res |
+                                 None \<Rightarrow> (map_of Globals x))"
+
+fun lookup_var :: "var_context \<Rightarrow> 'a nstate \<Rightarrow> vname \<Rightarrow> 'a val option"
+  where 
+   "lookup_var (Globals, Locals) ns x = 
+      (case (map_of Locals x) of Some res \<Rightarrow> local_state ns x |
+                                 None \<Rightarrow> global_state ns x)"
+
+(* if variable does not exist, then global state is updated *)
+fun update_var :: "var_context \<Rightarrow> 'a nstate \<Rightarrow> vname \<Rightarrow> 'a val \<Rightarrow>  'a nstate"
+  where 
+   "update_var (Globals, Locals) n_s x v =
+            (case (map_of Locals x) of Some res \<Rightarrow> n_s\<lparr>local_state := local_state(n_s)(x \<mapsto> v)\<rparr>  |
+                                 None \<Rightarrow> n_s\<lparr>global_state := global_state(n_s)(x \<mapsto> v) \<rparr>)"
 
 fun binop_less :: "lit \<Rightarrow> lit \<rightharpoonup> lit"
   where
@@ -143,82 +172,90 @@ fun instantiate :: "rtype_env \<Rightarrow> ty \<Rightarrow> ty"
   | "instantiate \<Omega> (TCon tcon_id ty_args) = (TCon tcon_id (map (instantiate \<Omega>) ty_args))"
 
 lemma instantiate_nil [simp]: "instantiate [] \<tau> = \<tau>"
-  by (induction \<tau>) (simp_all add: map_idI) 
+  by (induction \<tau>) (simp_all add: map_idI)
+
+fun full_ext_env :: "'a nstate \<Rightarrow> 'a val \<Rightarrow> 'a nstate"
+  where "full_ext_env n_s v = n_s\<lparr> binder_state := ext_env (binder_state n_s) v \<rparr>"
 
 (* big-step *)
-inductive red_expr :: "'a absval_ty_fun \<Rightarrow> 'a fun_context \<Rightarrow> rtype_env \<Rightarrow> expr \<Rightarrow> 'a nstate \<Rightarrow> 'a val \<Rightarrow> bool"
-  ("_,_,_ \<turnstile> ((\<langle>_,_\<rangle>) \<Down> _)" [51,0,0,0,0,0] 81)
-  and red_exprs :: "'a absval_ty_fun \<Rightarrow> 'a fun_context \<Rightarrow> rtype_env \<Rightarrow> expr list \<Rightarrow> 'a nstate \<Rightarrow> 'a val list \<Rightarrow> bool"
-  ("_,_,_ \<turnstile> ((\<langle>_,_\<rangle>) [\<Down>] _)" [51,0,0,0,0,0] 81)
-  for A :: "'a absval_ty_fun" and \<Gamma> :: "'a fun_context"
+inductive red_expr :: "'a absval_ty_fun \<Rightarrow> var_context \<Rightarrow> 'a fun_context \<Rightarrow> rtype_env \<Rightarrow> expr \<Rightarrow> 'a nstate \<Rightarrow> 'a val \<Rightarrow> bool"
+  ("_,_,_,_ \<turnstile> ((\<langle>_,_\<rangle>) \<Down> _)" [51,0,0,0,0,0] 81)
+  and red_exprs :: "'a absval_ty_fun \<Rightarrow> var_context \<Rightarrow> 'a fun_context \<Rightarrow> rtype_env \<Rightarrow> expr list \<Rightarrow> 'a nstate \<Rightarrow> 'a val list \<Rightarrow> bool"
+  ("_,_,_,_ \<turnstile> ((\<langle>_,_\<rangle>) [\<Down>] _)" [51,0,0,0,0,0] 81)
+  for A :: "'a absval_ty_fun" and \<Lambda> :: "var_context" and \<Gamma> :: "'a fun_context"
   where 
-    RedVar: "\<lbrakk> n_s(x) = Some v \<rbrakk> \<Longrightarrow> A,\<Gamma>,\<Omega> \<turnstile> \<langle>(Var x), n_s\<rangle> \<Down> v"
-  | RedLit: "A,\<Gamma>,\<Omega> \<turnstile> \<langle>(Lit v), n_s\<rangle> \<Down> LitV v" 
-  | RedBinOp: "\<lbrakk>A,\<Gamma>,\<Omega> \<turnstile> \<langle>e1, n_s\<rangle> \<Down> v1; A,\<Gamma>,\<Omega> \<turnstile> \<langle>e2, n_s\<rangle> \<Down> v2;
+    RedVar: "\<lbrakk> lookup_var \<Lambda> n_s x = Some v \<rbrakk> \<Longrightarrow> A,\<Lambda>,\<Gamma>,\<Omega> \<turnstile> \<langle>(Var x), n_s\<rangle> \<Down> v"
+  | RedBVar: "\<lbrakk> binder_state n_s i = Some v \<rbrakk> \<Longrightarrow> A,\<Lambda>,\<Gamma>,\<Omega> \<turnstile> \<langle>BVar i, n_s\<rangle> \<Down> v"
+  | RedLit: "A,\<Lambda>,\<Gamma>,\<Omega> \<turnstile> \<langle>(Lit v), n_s\<rangle> \<Down> LitV v" 
+  | RedBinOp: "\<lbrakk>A,\<Lambda>,\<Gamma>,\<Omega> \<turnstile> \<langle>e1, n_s\<rangle> \<Down> v1; A,\<Lambda>,\<Gamma>,\<Omega> \<turnstile> \<langle>e2, n_s\<rangle> \<Down> v2;
                  binop_eval_val bop v1 v2 = (Some v) \<rbrakk> \<Longrightarrow> 
-             A,\<Gamma>,\<Omega> \<turnstile> \<langle>(e1 \<guillemotleft>bop\<guillemotright> e2), n_s\<rangle> \<Down> v"
-  | RedUnOp: " \<lbrakk> A,\<Gamma>,\<Omega> \<turnstile> \<langle>e, n_s\<rangle> \<Down> v; unop_eval_val uop v = Some v' \<rbrakk> \<Longrightarrow> A,\<Gamma>,\<Omega> \<turnstile> \<langle>UnOp uop e, n_s\<rangle> \<Down> v'"
+             A,\<Lambda>,\<Gamma>,\<Omega> \<turnstile> \<langle>(e1 \<guillemotleft>bop\<guillemotright> e2), n_s\<rangle> \<Down> v"
+  | RedUnOp: " \<lbrakk> A,\<Lambda>,\<Gamma>,\<Omega> \<turnstile> \<langle>e, n_s\<rangle> \<Down> v; unop_eval_val uop v = Some v' \<rbrakk> \<Longrightarrow> A,\<Lambda>,\<Gamma>,\<Omega> \<turnstile> \<langle>UnOp uop e, n_s\<rangle> \<Down> v'"
   | RedFunOp: "\<lbrakk>(snd \<Gamma>) f = Some f_interp;
-                A,\<Gamma>,\<Omega> \<turnstile> \<langle>args, n_s\<rangle> [\<Down>] v_args;
+                A,\<Lambda>,\<Gamma>,\<Omega> \<turnstile> \<langle>args, n_s\<rangle> [\<Down>] v_args;
                 f_interp (map (instantiate \<Omega>) ty_args) v_args = Some v \<rbrakk> \<Longrightarrow>
-             A,\<Gamma>,\<Omega> \<turnstile> \<langle> FunExp f ty_args args, n_s \<rangle> \<Down> v"
+             A,\<Lambda>,\<Gamma>,\<Omega> \<turnstile> \<langle> FunExp f ty_args args, n_s \<rangle> \<Down> v"
+  | RedOld: "\<lbrakk> A,\<Lambda>,\<Gamma>,\<Omega> \<turnstile> \<langle> e, n_s\<lparr>global_state := old_global_state n_s \<rparr> \<rangle> \<Down> v\<rbrakk> \<Longrightarrow> 
+            A,\<Lambda>,\<Gamma>,\<Omega> \<turnstile> \<langle> Old e, n_s \<rangle> \<Down> v"
   | RedExpListNil:
-    "A,\<Gamma>,\<Omega> \<turnstile> \<langle>[], n_s\<rangle> [\<Down>] []"
+    "A,\<Lambda>,\<Gamma>,\<Omega> \<turnstile> \<langle>[], n_s\<rangle> [\<Down>] []"
   | RedExpListCons:
-    "\<lbrakk>A,\<Gamma>,\<Omega> \<turnstile> \<langle>e, n_s\<rangle> \<Down> v; A,\<Gamma>,\<Omega> \<turnstile> \<langle>es, n_s\<rangle> [\<Down>] vs \<rbrakk> \<Longrightarrow>
-      A,\<Gamma>,\<Omega> \<turnstile> \<langle>(e # es), n_s\<rangle> [\<Down>] (v # vs)"
+    "\<lbrakk>A,\<Lambda>,\<Gamma>,\<Omega> \<turnstile> \<langle>e, n_s\<rangle> \<Down> v; A,\<Lambda>,\<Gamma>,\<Omega> \<turnstile> \<langle>es, n_s\<rangle> [\<Down>] vs \<rbrakk> \<Longrightarrow>
+      A,\<Lambda>,\<Gamma>,\<Omega> \<turnstile> \<langle>(e # es), n_s\<rangle> [\<Down>] (v # vs)"
 (* value quantification rules *)
   | RedForAllTrue:
-    "\<lbrakk>\<And>v. type_of_val A v = (instantiate \<Omega> ty) \<Longrightarrow> A,\<Gamma>,\<Omega> \<turnstile> \<langle>e, ext_env n_s v\<rangle> \<Down> LitV (LBool True) \<rbrakk> \<Longrightarrow> 
-     A,\<Gamma>,\<Omega> \<turnstile> \<langle>Forall ty e, n_s\<rangle> \<Down> LitV (LBool True)"
+    "\<lbrakk>\<And>v. type_of_val A v = (instantiate \<Omega> ty) \<Longrightarrow> A,\<Lambda>,\<Gamma>,\<Omega> \<turnstile> \<langle>e, full_ext_env n_s v\<rangle> \<Down> LitV (LBool True) \<rbrakk> \<Longrightarrow> 
+     A,\<Lambda>,\<Gamma>,\<Omega> \<turnstile> \<langle>Forall ty e, n_s\<rangle> \<Down> LitV (LBool True)"
   | RedForAllFalse:
-    "\<lbrakk>type_of_val A v = instantiate \<Omega> ty; A,\<Gamma>,\<Omega> \<turnstile> \<langle>e, ext_env n_s v\<rangle> \<Down> LitV (LBool False) \<rbrakk> \<Longrightarrow> 
-     A,\<Gamma>,\<Omega> \<turnstile> \<langle>Forall ty e, n_s\<rangle> \<Down> LitV (LBool False)"
+    "\<lbrakk>type_of_val A v = instantiate \<Omega> ty; A,\<Lambda>,\<Gamma>,\<Omega> \<turnstile> \<langle>e, full_ext_env n_s v\<rangle> \<Down> LitV (LBool False) \<rbrakk> \<Longrightarrow> 
+     A,\<Lambda>,\<Gamma>,\<Omega> \<turnstile> \<langle>Forall ty e, n_s\<rangle> \<Down> LitV (LBool False)"
   | RedExistsTrue:
-    "\<lbrakk>type_of_val A v = instantiate \<Omega> ty; A,\<Gamma>,\<Omega> \<turnstile> \<langle>e, ext_env n_s v\<rangle> \<Down> LitV (LBool True) \<rbrakk> \<Longrightarrow>
-     A,\<Gamma>,\<Omega> \<turnstile> \<langle>Exists ty e, n_s\<rangle> \<Down> LitV (LBool True)"
+    "\<lbrakk>type_of_val A v = instantiate \<Omega> ty; A,\<Lambda>,\<Gamma>,\<Omega> \<turnstile> \<langle>e, full_ext_env n_s v\<rangle> \<Down> LitV (LBool True) \<rbrakk> \<Longrightarrow>
+     A,\<Lambda>,\<Gamma>,\<Omega> \<turnstile> \<langle>Exists ty e, n_s\<rangle> \<Down> LitV (LBool True)"
   | RedExistsFalse:
-    "\<lbrakk>\<And>v. type_of_val A v = instantiate \<Omega> ty \<Longrightarrow> A,\<Gamma>,\<Omega> \<turnstile> \<langle>e, ext_env n_s v\<rangle> \<Down> LitV (LBool False) \<rbrakk> \<Longrightarrow>
-     A,\<Gamma>,\<Omega> \<turnstile> \<langle>Exists ty e, n_s\<rangle> \<Down> LitV (LBool False)"
+    "\<lbrakk>\<And>v. type_of_val A v = instantiate \<Omega> ty \<Longrightarrow> A,\<Lambda>,\<Gamma>,\<Omega> \<turnstile> \<langle>e, full_ext_env n_s v\<rangle> \<Down> LitV (LBool False) \<rbrakk> \<Longrightarrow>
+     A,\<Lambda>,\<Gamma>,\<Omega> \<turnstile> \<langle>Exists ty e, n_s\<rangle> \<Down> LitV (LBool False)"
 (* type quantification rules *)
   | RedForallT_True:
-    "\<lbrakk>\<And>\<tau>. closed \<tau> \<Longrightarrow> A,\<Gamma>,(\<tau>#\<Omega>) \<turnstile> \<langle>e, n_s\<rangle> \<Down> LitV (LBool True) \<rbrakk> \<Longrightarrow> 
-     A,\<Gamma>,\<Omega> \<turnstile> \<langle>ForallT e, n_s\<rangle> \<Down> LitV (LBool True)"
+    "\<lbrakk>\<And>\<tau>. closed \<tau> \<Longrightarrow> A,\<Lambda>,\<Gamma>,(\<tau>#\<Omega>) \<turnstile> \<langle>e, n_s\<rangle> \<Down> LitV (LBool True) \<rbrakk> \<Longrightarrow> 
+     A,\<Lambda>,\<Gamma>,\<Omega> \<turnstile> \<langle>ForallT e, n_s\<rangle> \<Down> LitV (LBool True)"
   | RedForallT_False:
-    "\<lbrakk>closed \<tau>; A,\<Gamma>,(\<tau>#\<Omega>) \<turnstile> \<langle>e, n_s\<rangle> \<Down> LitV (LBool False) \<rbrakk> \<Longrightarrow>
-     A,\<Gamma>,\<Omega> \<turnstile> \<langle>ForallT e, n_s\<rangle> \<Down> LitV (LBool False)"
+    "\<lbrakk>closed \<tau>; A,\<Lambda>,\<Gamma>,(\<tau>#\<Omega>) \<turnstile> \<langle>e, n_s\<rangle> \<Down> LitV (LBool False) \<rbrakk> \<Longrightarrow>
+     A,\<Lambda>,\<Gamma>,\<Omega> \<turnstile> \<langle>ForallT e, n_s\<rangle> \<Down> LitV (LBool False)"
   | RedExistsT_True:
-    "\<lbrakk>closed \<tau>; A,\<Gamma>,(\<tau>#\<Omega>) \<turnstile> \<langle>e, n_s\<rangle> \<Down> LitV (LBool True) \<rbrakk> \<Longrightarrow>
-     A,\<Gamma>,\<Omega> \<turnstile> \<langle>ExistsT e, n_s\<rangle> \<Down> LitV (LBool True)"
+    "\<lbrakk>closed \<tau>; A,\<Lambda>,\<Gamma>,(\<tau>#\<Omega>) \<turnstile> \<langle>e, n_s\<rangle> \<Down> LitV (LBool True) \<rbrakk> \<Longrightarrow>
+     A,\<Lambda>,\<Gamma>,\<Omega> \<turnstile> \<langle>ExistsT e, n_s\<rangle> \<Down> LitV (LBool True)"
   | RedExistsT_False:
-    "\<lbrakk>\<And>\<tau>. closed \<tau> \<Longrightarrow> A,\<Gamma>,(\<tau>#\<Omega>) \<turnstile> \<langle>e, n_s\<rangle> \<Down> LitV (LBool False) \<rbrakk> \<Longrightarrow>
-     A,\<Gamma>,\<Omega> \<turnstile> \<langle>ExistsT e, n_s\<rangle> \<Down> LitV (LBool False)"
+    "\<lbrakk>\<And>\<tau>. closed \<tau> \<Longrightarrow> A,\<Lambda>,\<Gamma>,(\<tau>#\<Omega>) \<turnstile> \<langle>e, n_s\<rangle> \<Down> LitV (LBool False) \<rbrakk> \<Longrightarrow>
+     A,\<Lambda>,\<Gamma>,\<Omega> \<turnstile> \<langle>ExistsT e, n_s\<rangle> \<Down> LitV (LBool False)"
 
-inductive_cases RedBinOp_case[elim!]: "A,\<Gamma>,\<Omega> \<turnstile> \<langle>(e1 \<guillemotleft>bop\<guillemotright> e2), n_s\<rangle> \<Down> v"
-inductive_cases RedUnOp_case[elim!]: "A,\<Gamma>,\<Omega> \<turnstile> \<langle>UnOp uop e1, n_s\<rangle> \<Down> v"
-inductive_cases RedFunOp_case[elim!]: "A,\<Gamma>,\<Omega> \<turnstile> \<langle> FunExp f ty_args args, n_s \<rangle> \<Down> v"
-inductive_cases RedLit_case[elim]: "A,\<Gamma>,\<Omega> \<turnstile> \<langle>(Lit l), n_s\<rangle> \<Down> LitV l"
-inductive_cases RedVar_case[elim!]: "A,\<Gamma>,\<Omega> \<turnstile> \<langle>(Var x), n_s\<rangle> \<Down> v"
-inductive_cases RedForallTrue_case: "A,\<Gamma>,\<Omega> \<turnstile> \<langle>Forall ty e, n_s\<rangle> \<Down> LitV (LBool True)"
-inductive_cases RedForallFalse_case: "A,\<Gamma>,\<Omega> \<turnstile> \<langle>Forall ty e, n_s\<rangle> \<Down> LitV (LBool False)"
+inductive_cases RedBinOp_case[elim!]: "A,\<Lambda>,\<Gamma>,\<Omega> \<turnstile> \<langle>(e1 \<guillemotleft>bop\<guillemotright> e2), n_s\<rangle> \<Down> v"
+inductive_cases RedUnOp_case[elim!]: "A,\<Lambda>,\<Gamma>,\<Omega> \<turnstile> \<langle>UnOp uop e1, n_s\<rangle> \<Down> v"
+inductive_cases RedFunOp_case[elim!]: "A,\<Lambda>,\<Gamma>,\<Omega> \<turnstile> \<langle> FunExp f ty_args args, n_s \<rangle> \<Down> v"
+inductive_cases RedLit_case[elim]: "A,\<Lambda>,\<Gamma>,\<Omega> \<turnstile> \<langle>(Lit l), n_s\<rangle> \<Down> LitV l"
+inductive_cases RedVar_case[elim!]: "A,\<Lambda>,\<Gamma>,\<Omega> \<turnstile> \<langle>(Var x), n_s\<rangle> \<Down> v"
+inductive_cases RedForallTrue_case: "A,\<Lambda>,\<Gamma>,\<Omega> \<turnstile> \<langle>Forall ty e, n_s\<rangle> \<Down> LitV (LBool True)"
+inductive_cases RedForallFalse_case: "A,\<Lambda>,\<Gamma>,\<Omega> \<turnstile> \<langle>Forall ty e, n_s\<rangle> \<Down> LitV (LBool False)"
+
 
 inductive red_cmd :: "'a absval_ty_fun \<Rightarrow> var_context \<Rightarrow> 'a fun_context \<Rightarrow>rtype_env \<Rightarrow> cmd \<Rightarrow> 'a state \<Rightarrow> 'a state \<Rightarrow> bool"
   ("_,_,_,_ \<turnstile> ((\<langle>_,_\<rangle>) \<rightarrow>/ _)" [51,51,0,0,0] 81)
   for A :: "'a absval_ty_fun" and \<Lambda> :: var_context and  \<Gamma> :: "'a fun_context" and \<Omega> :: rtype_env
   where
-    RedAssertOk: "\<lbrakk> A,\<Gamma>,\<Omega> \<turnstile> \<langle>e, n_s\<rangle> \<Down> LitV (LBool True) \<rbrakk> \<Longrightarrow> 
+    RedAssertOk: "\<lbrakk> A,\<Lambda>,\<Gamma>,\<Omega> \<turnstile> \<langle>e, n_s\<rangle> \<Down> LitV (LBool True) \<rbrakk> \<Longrightarrow> 
                  A,\<Lambda>,\<Gamma>,\<Omega> \<turnstile> \<langle>Assert e, Normal n_s\<rangle> \<rightarrow> Normal n_s"
-  | RedAssertFail: "\<lbrakk> A,\<Gamma>,\<Omega> \<turnstile> \<langle>e, n_s\<rangle> \<Down> LitV (LBool False) \<rbrakk> \<Longrightarrow> 
+  | RedAssertFail: "\<lbrakk> A,\<Lambda>,\<Gamma>,\<Omega> \<turnstile> \<langle>e, n_s\<rangle> \<Down> LitV (LBool False) \<rbrakk> \<Longrightarrow> 
                   A,\<Lambda>,\<Gamma>,\<Omega> \<turnstile> \<langle>Assert e, Normal n_s\<rangle> \<rightarrow> Failure"
-  | RedAssumeOk: "\<lbrakk> A,\<Gamma>,\<Omega> \<turnstile> \<langle>e, n_s\<rangle> \<Down> LitV (LBool True) \<rbrakk> \<Longrightarrow> 
+  | RedAssumeOk: "\<lbrakk> A,\<Lambda>,\<Gamma>,\<Omega> \<turnstile> \<langle>e, n_s\<rangle> \<Down> LitV (LBool True) \<rbrakk> \<Longrightarrow> 
                 A,\<Lambda>,\<Gamma>,\<Omega> \<turnstile> \<langle>Assume e, Normal n_s\<rangle> \<rightarrow> Normal n_s"
-  | RedAssumeMagic: "\<lbrakk> A,\<Gamma>,\<Omega> \<turnstile> \<langle>e, n_s\<rangle> \<Down> LitV (LBool False) \<rbrakk> \<Longrightarrow> 
+  | RedAssumeMagic: "\<lbrakk> A,\<Lambda>,\<Gamma>,\<Omega> \<turnstile> \<langle>e, n_s\<rangle> \<Down> LitV (LBool False) \<rbrakk> \<Longrightarrow> 
                 A,\<Lambda>,\<Gamma>,\<Omega> \<turnstile> \<langle>Assume e, Normal n_s\<rangle> \<rightarrow> Magic"
-  | RedAssign: "\<lbrakk>A,\<Gamma>,\<Omega> \<turnstile> \<langle>(map snd upds), n_s\<rangle> [\<Down>] vs \<rbrakk> \<Longrightarrow>
-               A,\<Lambda>,\<Gamma>,\<Omega> \<turnstile> \<langle>Assign upds, Normal n_s\<rangle> \<rightarrow>  Normal (n_s((map fst upds) [\<mapsto>] vs))"  
+(* multi-assign not supported for now *)
+  | RedAssign: "\<lbrakk>A,\<Lambda>,\<Gamma>,\<Omega> \<turnstile> \<langle>e, n_s\<rangle> \<Down> v \<rbrakk> \<Longrightarrow>
+               A,\<Lambda>,\<Gamma>,\<Omega> \<turnstile> \<langle>Assign x e, Normal n_s\<rangle> \<rightarrow>  Normal (update_var \<Lambda> n_s x v)"  
 (* restrict x < length \<Lambda> ? *)
-  | RedHavoc: "\<lbrakk> (\<Lambda> ! x) = ty; type_of_val A v = ty \<rbrakk> \<Longrightarrow>
-               A,\<Lambda>,\<Gamma>,\<Omega> \<turnstile> \<langle>Havoc x, Normal n_s\<rangle> \<rightarrow> Normal (n_s(x \<mapsto> v))"
+  | RedHavoc: "\<lbrakk> lookup_var_ty \<Lambda> x  = Some ty; type_of_val A v = ty \<rbrakk> \<Longrightarrow>
+               A,\<Lambda>,\<Gamma>,\<Omega> \<turnstile> \<langle>Havoc x, Normal n_s\<rangle> \<rightarrow> Normal (update_var \<Lambda> n_s x v)"
   | RedPropagateMagic: "A,\<Lambda>,\<Gamma>,\<Omega> \<turnstile> \<langle>s, Magic\<rangle> \<rightarrow> Magic"
   | RedPropagateFailure: "A,\<Lambda>,\<Gamma>,\<Omega> \<turnstile> \<langle>s, Failure\<rangle> \<rightarrow> Failure"
 
@@ -278,20 +315,20 @@ definition fun_interp_wf :: "'a absval_ty_fun \<Rightarrow> fdecls \<Rightarrow>
             (\<forall>fn fd. map_of fds fn = Some fd \<longrightarrow> 
                   (\<exists>f. \<gamma>_interp fn = Some f \<and> fun_interp_single_wf A fd f \<and> fun_interp_single_wf_2 A fd f))"
 
-definition state_typ_wf :: "'a absval_ty_fun \<Rightarrow> rtype_env \<Rightarrow> 'a nstate \<Rightarrow> vdecls \<Rightarrow> bool"
+definition state_typ_wf :: "'a absval_ty_fun \<Rightarrow> rtype_env \<Rightarrow> 'a named_state \<Rightarrow> vdecls \<Rightarrow> bool"
   where "state_typ_wf A \<Omega> ns vs = 
-           (\<forall> v ty. vs ! v = ty  \<longrightarrow> 
+           (\<forall> v ty. map_of vs v = Some ty  \<longrightarrow> 
                           Option.map_option (\<lambda>v. type_of_val A v) (ns(v)) = (Some (instantiate \<Omega> ty)))"
 
-definition method_body_verifies :: "'a absval_ty_fun \<Rightarrow> vdecls \<Rightarrow> fdecls \<Rightarrow> 'a fun_interp \<Rightarrow> rtype_env \<Rightarrow> mbodyCFG \<Rightarrow> 'a nstate \<Rightarrow> bool"
+definition method_body_verifies :: "'a absval_ty_fun \<Rightarrow> var_context \<Rightarrow> fdecls \<Rightarrow> 'a fun_interp \<Rightarrow> rtype_env \<Rightarrow> mbodyCFG \<Rightarrow> 'a nstate \<Rightarrow> bool"
   where "method_body_verifies A vds fds \<gamma>_interp \<Omega> mbody ns = 
       (\<forall> m' s'. (A, vds, (fds, \<gamma>_interp), \<Omega>, mbody \<turnstile> (Inl (entry(mbody)), Normal ns) -n\<rightarrow>* (m',s')) \<longrightarrow> s' \<noteq> Failure)"
 
-definition axiom_sat :: "'a absval_ty_fun \<Rightarrow> 'a fun_context \<Rightarrow> 'a nstate \<Rightarrow> axiom \<Rightarrow> bool"
-  where "axiom_sat A \<Gamma> n_s a = (A,\<Gamma>,[] \<turnstile> \<langle>a, n_s\<rangle> \<Down> LitV (LBool True))"
+definition axiom_sat :: "'a absval_ty_fun \<Rightarrow> var_context \<Rightarrow> 'a fun_context \<Rightarrow> 'a nstate \<Rightarrow> axiom \<Rightarrow> bool"
+  where "axiom_sat A \<Lambda> \<Gamma> n_s a = (A,\<Lambda>,\<Gamma>,[] \<turnstile> \<langle>a, n_s\<rangle> \<Down> LitV (LBool True))"
 
-definition axioms_sat :: "'a absval_ty_fun \<Rightarrow> 'a fun_context \<Rightarrow> 'a nstate \<Rightarrow> axiom list \<Rightarrow> bool"
-  where "axioms_sat A \<Gamma> n_s as = list_all (axiom_sat A \<Gamma> n_s) as"
+definition axioms_sat :: "'a absval_ty_fun \<Rightarrow> var_context \<Rightarrow> 'a fun_context \<Rightarrow> 'a nstate \<Rightarrow> axiom list \<Rightarrow> bool"
+  where "axioms_sat A \<Lambda> \<Gamma> n_s as = list_all (axiom_sat A \<Lambda> \<Gamma> n_s) as"
 
 (* not most compact representation (dom ns =... implied by ... state_typ wf ... ) *)
 (* disjointness condition does not reflect Boogie which allows shadowing of global variables *)
@@ -300,33 +337,42 @@ fun method_verify :: "'a absval_ty_fun \<Rightarrow> prog \<Rightarrow> mdecl \<
     "method_verify A (Program tdecls fdecls consts gvars axioms mdecls) (mname, n_ty_params, args, locals, mbody) =
     ((\<forall>t. closed t \<longrightarrow> (\<exists>v. type_of_val A v = t)) \<longrightarrow>
     (\<forall> \<gamma>_interp. fun_interp_wf A fdecls \<gamma>_interp \<longrightarrow>
-     (\<forall>ns. 
-       (axioms_sat A (fdecls, \<gamma>_interp) ns axioms) \<longrightarrow>
-       (\<forall>\<Omega>. (list_all closed \<Omega> \<and> length \<Omega> = n_ty_params) \<longrightarrow>
-       (state_typ_wf A \<Omega> ns (args@locals@gvars@consts)) \<longrightarrow>
-        method_body_verifies A (args@locals@gvars@consts) fdecls \<gamma>_interp \<Omega> mbody ns )
+    (\<forall> \<Omega> gs. state_typ_wf A \<Omega> gs consts \<longrightarrow> 
+              (axioms_sat A (consts, []) (fdecls, \<gamma>_interp) \<lparr>old_global_state = Map.empty, global_state = gs, local_state = Map.empty, binder_state = Map.empty\<rparr> axioms)) \<longrightarrow>
+    (\<forall> gs. 
+       (\<forall> \<Omega>'. state_typ_wf A \<Omega>' gs gvars) \<longrightarrow>
+       (\<forall> \<Omega>'. state_typ_wf A \<Omega>' gs consts) \<longrightarrow>      
+       (\<forall>\<Omega> ls. (list_all closed \<Omega> \<and> length \<Omega> = n_ty_params) \<longrightarrow>
+       (state_typ_wf A \<Omega> ls args \<longrightarrow>
+        state_typ_wf A \<Omega> ls locals \<longrightarrow>
+        method_body_verifies A (gvars@consts, args@locals) fdecls \<gamma>_interp \<Omega> mbody \<lparr>old_global_state = gs, global_state = gs, local_state = ls, binder_state = Map.empty\<rparr> )
       )
-    ))"
+    )))"
 
 lemma expr_eval_determ: 
-shows "((A,\<Gamma>,\<Omega> \<turnstile> \<langle>e1, s\<rangle> \<Down> v) \<Longrightarrow> ((A,\<Gamma>,\<Omega> \<turnstile> \<langle>e1, s\<rangle> \<Down> v') \<Longrightarrow> v = v'))"  
-    and "(A,\<Gamma>,\<Omega> \<turnstile> \<langle>es, s\<rangle> [\<Down>] vs) \<Longrightarrow> (A,\<Gamma>,\<Omega> \<turnstile> \<langle>es, s\<rangle> [\<Down>] vs') \<Longrightarrow> vs = vs' "
+shows "((A,\<Lambda>,\<Gamma>,\<Omega> \<turnstile> \<langle>e1, s\<rangle> \<Down> v) \<Longrightarrow> ((A,\<Lambda>,\<Gamma>,\<Omega> \<turnstile> \<langle>e1, s\<rangle> \<Down> v') \<Longrightarrow> v = v'))"  
+    and "(A,\<Lambda>,\<Gamma>,\<Omega> \<turnstile> \<langle>es, s\<rangle> [\<Down>] vs) \<Longrightarrow> (A,\<Lambda>,\<Gamma>,\<Omega> \<turnstile> \<langle>es, s\<rangle> [\<Down>] vs') \<Longrightarrow> vs = vs' "
 proof (induction arbitrary: v' and vs' rule: red_expr_red_exprs.inducts)
   case (RedVar n_s x v \<Omega>)
-  assume "n_s x = Some v"
-  assume "A,\<Gamma>,\<Omega> \<turnstile> \<langle>Var x,n_s\<rangle> \<Down> v'"
-  then show ?case using \<open>n_s x = Some v\<close> by (cases; simp)
+  assume "lookup_var \<Lambda> n_s x = Some v"
+  assume "A,\<Lambda>,\<Gamma>,\<Omega> \<turnstile> \<langle>Var x,n_s\<rangle> \<Down> v'"
+  then show ?case using \<open>lookup_var \<Lambda> n_s x = Some v\<close> by (cases; simp)
+next
+  case (RedBVar n_s i v \<Omega>)
+  assume "binder_state n_s i = Some v"
+  assume "A,\<Lambda>,\<Gamma>,\<Omega> \<turnstile> \<langle>BVar i,n_s\<rangle> \<Down> v'"
+  then show ?case using \<open>binder_state n_s i = Some v\<close> by (cases; simp)
 next
   case (RedLit \<Omega> l n_s)
-  assume "A,\<Gamma>,\<Omega> \<turnstile> \<langle>Lit l,n_s\<rangle> \<Down> v'"
+  assume "A,\<Lambda>,\<Gamma>,\<Omega> \<turnstile> \<langle>Lit l,n_s\<rangle> \<Down> v'"
   then show ?case by (cases; simp)
 next
   case (RedBinOp \<Omega> e1 n_s v1 e2 v2 bop v)
   from RedBinOp.prems show ?case
   proof (cases)
     fix v1' v2'
-    assume "A,\<Gamma>,\<Omega> \<turnstile> \<langle>e1,n_s\<rangle> \<Down> v1'" hence "v1 = v1'" using RedBinOp.IH by simp
-    assume "A,\<Gamma>,\<Omega> \<turnstile> \<langle>e2,n_s\<rangle> \<Down> v2'" hence "v2 = v2'" using RedBinOp.IH by simp
+    assume "A,\<Lambda>,\<Gamma>,\<Omega> \<turnstile> \<langle>e1,n_s\<rangle> \<Down> v1'" hence "v1 = v1'" using RedBinOp.IH by simp
+    assume "A,\<Lambda>,\<Gamma>,\<Omega> \<turnstile> \<langle>e2,n_s\<rangle> \<Down> v2'" hence "v2 = v2'" using RedBinOp.IH by simp
     assume "binop_eval_val bop v1' v2' = Some v'"
     with \<open>v1 = v1'\<close> \<open>v2 = v2'\<close> show ?thesis using RedBinOp.hyps by simp
   qed
@@ -335,7 +381,7 @@ next
   from RedUnOp.prems show ?case
   proof (cases)
     fix v2
-    assume "A,\<Gamma>,\<Omega> \<turnstile> \<langle>e,n_s\<rangle> \<Down> v2" hence "v2 = v" using RedUnOp.IH by simp
+    assume "A,\<Lambda>,\<Gamma>,\<Omega> \<turnstile> \<langle>e,n_s\<rangle> \<Down> v2" hence "v2 = v" using RedUnOp.IH by simp
     assume "unop_eval_val uop v2 = Some veval"
     with \<open>v2 = v\<close> show ?thesis using RedUnOp.hyps by simp
   qed
@@ -344,7 +390,7 @@ next
   from RedFunOp.prems show ?case
   proof (cases)
     fix v_args' f_interp'
-    assume "A,\<Gamma>,\<Omega> \<turnstile> \<langle>args,n_s\<rangle> [\<Down>] v_args'" hence "v_args = v_args'" using RedFunOp.IH by simp
+    assume "A,\<Lambda>,\<Gamma>,\<Omega> \<turnstile> \<langle>args,n_s\<rangle> [\<Down>] v_args'" hence "v_args = v_args'" using RedFunOp.IH by simp
     assume "snd \<Gamma> f = Some f_interp'" hence "f_interp = f_interp'" using RedFunOp.IH by simp
     assume "f_interp' (map (instantiate \<Omega>) ty_args) v_args' = Some v'"
     thus ?case using \<open>v_args = v_args'\<close> \<open>f_interp = f_interp'\<close> using RedFunOp.hyps by simp
@@ -354,15 +400,18 @@ next
   thus ?case by (cases; simp)
 next
   case (RedExpListCons \<Omega> e n_s v es vs' vs'')
-  assume "A,\<Gamma>,\<Omega> \<turnstile> \<langle>e # es,n_s\<rangle> [\<Down>] vs''"
+  assume "A,\<Lambda>,\<Gamma>,\<Omega> \<turnstile> \<langle>e # es,n_s\<rangle> [\<Down>] vs''"
   thus ?case 
   proof cases
     fix w ws      
-    assume "A,\<Gamma>,\<Omega> \<turnstile> \<langle>e,n_s\<rangle> \<Down> w" hence "v = w" using RedExpListCons.IH by simp
-    assume "A,\<Gamma>,\<Omega> \<turnstile> \<langle>es,n_s\<rangle> [\<Down>] ws" hence "ws = vs'" using RedExpListCons.IH by simp  
+    assume "A,\<Lambda>,\<Gamma>,\<Omega> \<turnstile> \<langle>e,n_s\<rangle> \<Down> w" hence "v = w" using RedExpListCons.IH by simp
+    assume "A,\<Lambda>,\<Gamma>,\<Omega> \<turnstile> \<langle>es,n_s\<rangle> [\<Down>] ws" hence "ws = vs'" using RedExpListCons.IH by simp  
     moreover assume "vs'' = w # ws"
     ultimately show ?thesis using \<open>v = w\<close>  by simp
   qed
+next
+  case (RedOld \<Omega> e n_s v) 
+  thus ?case by (blast elim: red_expr.cases)
 next
   case (RedForAllTrue ty e n_s v')
   thus ?case by (blast elim: red_expr.cases)
@@ -389,7 +438,7 @@ next
   thus ?case by (blast elim: red_expr.cases)    
 qed
 
-lemma red_exprs_length: "A,\<Gamma>,\<Omega> \<turnstile> \<langle>es, n_s\<rangle> [\<Down>] vs \<Longrightarrow> length es = length vs"
+lemma red_exprs_length: "A,\<Lambda>,\<Gamma>,\<Omega> \<turnstile> \<langle>es, n_s\<rangle> [\<Down>] vs \<Longrightarrow> length es = length vs"
   by (induction vs arbitrary: es; erule red_exprs.cases; simp)
    
 lemma step_nil_same:
@@ -477,8 +526,8 @@ next
 qed
 
 lemma forall_red:
-  assumes "A, \<Gamma>, \<Omega> \<turnstile> \<langle>Forall ty e, n_s\<rangle> \<Down> v"
-  shows "\<exists>b. (v = LitV (LBool b)) \<and> (b = (\<forall>v'. type_of_val A v' = (instantiate \<Omega> ty) \<longrightarrow> A, \<Gamma>, \<Omega> \<turnstile> \<langle>e, ext_env n_s v'\<rangle> \<Down> LitV (LBool True)))"
+  assumes "A, \<Lambda>, \<Gamma>, \<Omega> \<turnstile> \<langle>Forall ty e, n_s\<rangle> \<Down> v"
+  shows "\<exists>b. (v = LitV (LBool b)) \<and> (b = (\<forall>v'. type_of_val A v' = (instantiate \<Omega> ty) \<longrightarrow> A, \<Lambda>, \<Gamma>, \<Omega> \<turnstile> \<langle>e, full_ext_env n_s v'\<rangle> \<Down> LitV (LBool True)))"
   using assms
 proof (cases)
   case RedForAllTrue
@@ -490,8 +539,8 @@ next
 qed
 
 lemma exists_red:
-  assumes "A, \<Gamma>, \<Omega> \<turnstile> \<langle>Exists ty e, n_s\<rangle> \<Down> v"
-  shows "\<exists>b. (v = LitV (LBool b)) \<and> (b = (\<exists>v'. (type_of_val A v' = (instantiate \<Omega> ty)) \<and> A,\<Gamma>,\<Omega> \<turnstile> \<langle>e, ext_env n_s v'\<rangle> \<Down> LitV (LBool True)))"
+  assumes "A, \<Lambda>, \<Gamma>, \<Omega> \<turnstile> \<langle>Exists ty e, n_s\<rangle> \<Down> v"
+  shows "\<exists>b. (v = LitV (LBool b)) \<and> (b = (\<exists>v'. (type_of_val A v' = (instantiate \<Omega> ty)) \<and> A,\<Lambda>,\<Gamma>,\<Omega> \<turnstile> \<langle>e, full_ext_env n_s v'\<rangle> \<Down> LitV (LBool True)))"
   using assms
 proof (cases)
   case RedExistsTrue
@@ -504,14 +553,14 @@ qed
 
 (* TODO: make more precise *)
 lemma forallt_red_bool:
-  assumes "A, \<Gamma>, \<Omega> \<turnstile> \<langle>ForallT e, n_s\<rangle> \<Down> v"
+  assumes "A, \<Lambda>, \<Gamma>, \<Omega> \<turnstile> \<langle>ForallT e, n_s\<rangle> \<Down> v"
   shows "\<exists>b. (v = LitV (LBool b))"
   using assms
   by (cases; auto)
 
 (* TODO: make more precise *)
 lemma existst_red_bool:
-  assumes "A, \<Gamma>, \<Omega> \<turnstile> \<langle>ExistsT e, n_s\<rangle> \<Down> v"
+  assumes "A, \<Lambda>, \<Gamma>, \<Omega> \<turnstile> \<langle>ExistsT e, n_s\<rangle> \<Down> v"
   shows "\<exists>b. (v = LitV (LBool b))"
   using assms
   by (cases; auto)
